tools/Vale/test/Vale.fst
@@ -45,14 +45,14 @@ let va_is_src_shift_amt_uint64 (o:operand) (s:va_state) = valid_shift_operand o 
 
 (* Getters *)
 let va_get_ok (s:va_state) :bool = s.ok
-let va_get_flags (s:va_state) :nat64 = s.flags
-let va_get_reg (r:reg) (s:va_state) :nat64 = eval_reg r s
+let va_get_flags (s:va_state) :int = FStar.UInt64.v s.flags
+let va_get_reg (r:reg) (s:va_state) :int = FStar.UInt64.v (eval_reg r s)
 let va_get_mem (s:va_state) :mem = s.mem
 
 (* Framing: va_update_foo means the two states are the same except for foo *)
 let va_update_ok (sM:va_state) (sK:va_state) :va_state  = { sK with ok = sM.ok }
 let va_update_flags  (sM:va_state) (sK:va_state) :va_state  = { sK with flags = sM.flags }
-let va_update_reg (r:reg) (sM:va_state) (sK:va_state) :va_state = { sK with regs = sK.regs.[r] <- va_get_reg r sM }
+let va_update_reg (r:reg) (sM:va_state) (sK:va_state) :va_state = { sK with regs = sK.regs.[r] <- (eval_reg r sM) }
 let va_update_mem (sM:va_state) (sK:va_state) :va_state = { sK with mem = sM.mem }
 let va_update_operand (o:operand) (sM:va_state) (sK:va_state) :va_state =
   match o with
@@ -63,12 +63,14 @@ let va_update_dst_operand (o:dst_op) (sM:va_state) (sK:va_state) :va_state =
   va_update_operand o sM sK   
 let va_update_register (r:reg) (sM:va_state) (sK:va_state) :va_state = va_update_reg r sM sK
 
+open FStar.UInt64
+
 (* Evaluation *)
-let va_eval_operand_uint64 (s:va_state) (o:va_operand) :nat64 = eval_operand o s
-let va_eval_dst_operand_uint64 (s:va_state) (o:va_dst_operand) :nat64 = eval_operand o s
-let va_eval_shift_amt_uint64 (s:va_state) (o:va_shift_amt) : nat64 = eval_operand o s
-let va_eval_cmp_uint64 (s:va_state) (r:va_cmp) :nat64 = eval_operand r s
-let va_eval_register_uint64 (s:va_state) (r:va_register) :nat64 = eval_reg r s
+let va_eval_operand_uint64 (s:va_state) (o:va_operand) :int = v (eval_operand o s)
+let va_eval_dst_operand_uint64 (s:va_state) (o:va_dst_operand) :int = v (eval_operand o s)
+let va_eval_shift_amt_uint64 (s:va_state) (o:va_shift_amt) : int = v (eval_operand o s)
+let va_eval_cmp_uint64 (s:va_state) (r:va_cmp) :int = v (eval_operand r s)
+let va_eval_register_uint64 (s:va_state) (r:va_register) :int = v (eval_reg r s)
 
 
 (* Dealing with code *)
@@ -131,9 +133,8 @@ let va_lemma_ifElse (ifb:ocmp) (ct:code) (cf:code) (s_0:va_state) (sN:va_state)
 
 let va_whileInv (b:ocmp) (c:code{While? c}) (inv:operand) (s_0:va_state) (sN:va_state) =
   let open FStar.UInt64 in
-  (v (eval_operand inv s_0) >= 0           /\
-  (forall (r:reg). s_0.regs `contains` r) /\
-  Some(sN) == eval_while c s_0)
+  va_eval_operand_uint64 s_0 inv >= 0 /\
+  Some(sN) == eval_while c s_0
 
 let va_lemma_while (b:ocmp) (c:code) (inv:operand) (s_0:va_state) (sN:va_state)
   :Pure va_state
@@ -141,11 +142,9 @@ let va_lemma_while (b:ocmp) (c:code) (inv:operand) (s_0:va_state) (sN:va_state)
 	(ensures  (fun s_1 -> Some(sN) == eval_while (While b c inv) s_0 /\ s_1 == s_0))
   = s_0
 
-open FStar.UInt64
-
 let va_lemma_whileTrue (b:ocmp) (c:code) (inv:operand) (s_0:va_state) (sN:va_state)
   :Pure (va_state * va_state)
-        (requires (v (eval_operand inv s_0) > 0 /\
+        (requires (va_eval_operand_uint64 s_0 inv > 0 /\
 	           Some(sN) == eval_while (While b c inv) s_0))
 	(ensures  (fun (s_0', s_1) -> s_0' == s_0         /\
 	                          eval_ocmp s_0 b      /\
